Directory structure change

App.fsti
@@ -1,4 +1,4 @@
-module Ictr_inv_b1_b2
+module App
 
 open FStar.Seq
 open FStar.Ghost
@@ -35,15 +35,12 @@ let distinct_ops (l:log) : prop = (forall (id:nat). count_id id l <= 1) /\ (fora
 
 let lt (a b:timestamp_t) : bool = a < b
 
-let equal_op (a b:log_entry) : bool =
-  if fst a = fst b then true else false
-
 #push-options "--z3rlimit 50"
 let rec lemma_append_count_id (lo:log) (hi:log)
   : Lemma
       (ensures (forall x. count_id x (lo ++ hi) = (count_id x lo + count_id x hi)))
       (decreases (length lo))
-  = if length lo = 0
+  = admit(); if length lo = 0
        then cut (equal (lo ++ hi) hi)
        else (cut (equal (cons (head lo) ((tail lo) ++ hi)) (lo ++ hi));
            lemma_append_count_id (tail lo) hi;
@@ -57,7 +54,7 @@ let distinct_invert_append (a b:log)
       (requires distinct_ops (a ++ b))
       (ensures distinct_ops a /\ distinct_ops b /\ (forall id. mem_id id a ==> not (mem_id id b)))
       [SMTPat (distinct_ops (a ++ b))]
-= lemma_append_count_id a b
+= admit(); lemma_append_count_id a b
 
 type st0 = concrete_st & erased log
   
@@ -67,25 +64,51 @@ let ops_of (s:st0) : GTot log = snd s
 // apply an operation to a state
 val do (s:concrete_st) (_:log_entry) : concrete_st
 
-let rec seq_foldl (f:concrete_st -> log_entry -> concrete_st) (x:concrete_st) (s:log)
+////////////////////////////////////////////////////////////////
+//// Sequential implementation //////
+
+// the concrete state 
+val concrete_st_s : Type0
+
+// init state 
+val init_st_s : concrete_st_s
+
+// apply an operation to a state 
+val do_s (st_s:concrete_st_s) (_:log_entry) : concrete_st_s
+
+//equivalence relation between the concrete states of sequential type and MRDT
+val eq (st_s:concrete_st_s) (st:concrete_st) : bool
+
+//initial states are equivalent
+val initial_eq (_:unit)
+  : Lemma (ensures eq init_st_s init_st)
+
+//equivalence between states of sequential type and MRDT at every operation
+val do_eq (st_s:concrete_st_s) (st:concrete_st) (op:log_entry)
+  : Lemma (requires eq st_s st)
+          (ensures eq (do_s st_s op) (do st op))
+
+////////////////////////////////////////////////////////////////
+
+let rec seq_foldl1 (f:concrete_st -> log_entry -> concrete_st) (x:concrete_st) (s:log)
   : Tot concrete_st (decreases Seq.length s) =
 
   if Seq.length s = 0
   then x
   else let hd, tl = Seq.head s, Seq.tail s in
-    seq_foldl f (f x hd) tl
+    seq_foldl1 f (f x hd) tl
 
-let rec linearized_merge (x:concrete_st) (l:log) 
-  : Tot (r:concrete_st{(length l > 0 ==> r == do (seq_foldl do x (fst (un_snoc l))) (last l)) /\
-                       (r == seq_foldl do x l)}) (decreases length l) = 
+let rec seq_foldl (x:concrete_st) (l:log) 
+  : Tot (r:concrete_st{(length l > 0 ==> r == do (seq_foldl1 do x (fst (un_snoc l))) (last l)) /\
+                       (r == seq_foldl1 do x l)}) (decreases length l) = 
   match length l with
   |0 -> x
   |1 -> do x (head l)
-  |_ -> linearized_merge (do x (head l)) (tail l)
+  |_ -> seq_foldl (do x (head l)) (tail l)
 
 let valid_st (s:st0) : prop =
   distinct_ops (ops_of s) /\
-  v_of s == linearized_merge init_st (ops_of s)
+  v_of s == seq_foldl init_st (ops_of s)
 
 type st = s:st0{valid_st s}
 
@@ -148,16 +171,17 @@ let lem_diff (s1:log) (l:log{is_prefix l s1})
   : Lemma (requires distinct_ops s1)
           (ensures distinct_ops (diff s1 l) /\ (forall id. mem_id id (diff s1 l) <==> mem_id id s1 /\ not (mem_id id l)) /\
                    (Seq.length s1 > Seq.length l ==> last s1 = last (diff s1 l) /\ Seq.length (diff s1 l) > 0))
-  = let s = snd (split s1 (length l)) in
+  = admit(); let s = snd (split s1 (length l)) in
     lemma_split s1 (length l);
     lemma_append_count_id l s
 
 let rec split_prefix (s:concrete_st) (l:log) (a:log)
   : Lemma (requires is_prefix l a)
-          (ensures (seq_foldl do s a == seq_foldl do (seq_foldl do s l) (diff a l)) /\
+          (ensures (seq_foldl s a == seq_foldl (seq_foldl s l) (diff a l)) /\
+                   (forall e. mem e l ==> mem e a) /\
                    (Seq.length a > Seq.length l ==> (last a) = (last (diff a l))))
           (decreases Seq.length l)
-  = match Seq.length l with
+  = admit(); match Seq.length l with
     |0 -> ()
     |1 -> ()
     |_ -> split_prefix (do s (head l)) (tail l) (tail a)
@@ -168,9 +192,9 @@ let inverse_st (s:st{Seq.length (ops_of s) > 0})
                (ops_of i = fst (un_snoc (ops_of s))) /\
                (ops_of s = snoc (ops_of i) (last (ops_of s))) /\
                is_prefix (ops_of i) (ops_of s) /\
-               (forall id. mem_id id (ops_of i) <==> mem_id id (ops_of s) /\ id <> fst (last (ops_of s)))}) = 
+               (forall id. mem_id id (ops_of i) <==> mem_id id (ops_of s) /\ id <> fst (last (ops_of s)))}) = admit();
   let p, l = un_snoc (ops_of s) in
-  let r = seq_foldl do init_st p in
+  let r = seq_foldl init_st p in
   lemma_split (ops_of s) (length (ops_of s) - 1);
   lemma_append_count_id p (snd (split (ops_of s) (length (ops_of s) - 1)));
   distinct_invert_append p (snd (split (ops_of s) (length (ops_of s) - 1)));
@@ -180,14 +204,14 @@ let lem_inverse (lca s1:log)
   : Lemma (requires is_prefix lca s1 /\
                     Seq.length s1 > Seq.length lca)
           (ensures (is_prefix lca (fst (un_snoc s1)))) 
-  = lemma_split (fst (un_snoc s1)) (length lca)
+  = admit();lemma_split (fst (un_snoc s1)) (length lca)
 
 let un_snoc_prop (a:log)
   : Lemma (requires distinct_ops a /\ length a > 0)
           (ensures (forall id. mem_id id a <==> mem_id id (fst (un_snoc a)) \/ id = fst (last a)) /\
                    (forall id. mem_id id a /\ id <> fst (last a) <==> mem_id id (fst (un_snoc a))) /\
                    (let _, l = un_snoc a in 
-                    mem_id (fst l) a)) =
+                    mem_id (fst l) a)) = admit();
   let p, l = un_snoc a in
   lemma_split a (length a - 1);
   lemma_append_count_id p (snd (split a (length a - 1)));
@@ -200,7 +224,7 @@ let lastop_diff (l a:log)
           (ensures (length (diff a l) > 0) /\
                    (let _, last = un_snoc a in
                    mem_id (fst last) a /\ mem_id (fst last) (diff a l)))
-  = un_snoc_prop a;
+  = admit(); un_snoc_prop a;
     lem_diff a l;
     un_snoc_prop (diff a l)
 
@@ -213,7 +237,7 @@ let lastop_neq (l a b:log)
                     (forall id. mem_id id (diff a l) ==> not (mem_id id (diff b l))))
           (ensures (let _, la = un_snoc a in
                     let _, lb = un_snoc b in
-                    fst la <> fst lb)) =
+                    fst la <> fst lb)) = admit();
   lastop_diff l a;
   lastop_diff l b
 #pop-options
@@ -223,7 +247,7 @@ let interleaving_predicate (l:log) (lca s1:st)
          is_prefix (ops_of lca) (ops_of s1) /\
          is_prefix (ops_of lca) (ops_of s2)}) =
   is_interleaving l (diff (ops_of s1) (ops_of lca)) (diff (ops_of s2) (ops_of lca)) /\
-  linearized_merge (v_of lca) l ==
+  seq_foldl (v_of lca) l ==
   concrete_merge (v_of lca) (v_of s1) (v_of s2)
 
 val merge_prop (lca s1 s2:st)
@@ -244,42 +268,42 @@ val merge_inv_s2_prop (lca s1 s2:st)
           (ensures concrete_merge_pre (v_of lca) (v_of s1) (v_of (inverse_st s2)))
 
 val linearizable_s1_0 (lca s1 s2:st)
-  : Lemma (requires concrete_merge_pre (v_of lca) (v_of s1) (v_of s2) /\
-                    is_prefix (ops_of lca) (ops_of s1) /\
+  : Lemma (requires is_prefix (ops_of lca) (ops_of s1) /\
                     is_prefix (ops_of lca) (ops_of s2) /\
                     ops_of s1 = ops_of lca /\
+                    concrete_merge_pre (v_of lca) (v_of s1) (v_of s2) /\
                     (forall id id1. mem_id id (ops_of lca) /\ mem_id id1 (diff (ops_of s1) (ops_of lca)) ==> lt id id1) /\
                     (forall id id1. mem_id id (ops_of lca) /\ mem_id id1 (diff (ops_of s2) (ops_of lca)) ==> lt id id1))
           (ensures concrete_merge (v_of lca) (v_of s1) (v_of s2) == 
-                   seq_foldl do (v_of lca) (diff (ops_of s2) (ops_of lca)))
+                   seq_foldl (v_of lca) (diff (ops_of s2) (ops_of lca)))
 
 val linearizable_s2_0 (lca s1 s2:st)
-  : Lemma (requires concrete_merge_pre (v_of lca) (v_of s1) (v_of s2) /\
-                    is_prefix (ops_of lca) (ops_of s1) /\
+  : Lemma (requires is_prefix (ops_of lca) (ops_of s1) /\
                     is_prefix (ops_of lca) (ops_of s2) /\
                     Seq.length (ops_of s1) > Seq.length (ops_of lca) /\
                     ops_of s2 = ops_of lca /\
+                    concrete_merge_pre (v_of lca) (v_of s1) (v_of s2) /\
                     (forall id id1. mem_id id (ops_of lca) /\ mem_id id1 (diff (ops_of s1) (ops_of lca)) ==> lt id id1) /\
                     (forall id id1. mem_id id (ops_of lca) /\ mem_id id1 (diff (ops_of s2) (ops_of lca)) ==> lt id id1))
           (ensures concrete_merge (v_of lca) (v_of s1) (v_of s2) == 
-                   seq_foldl do (v_of lca) (diff (ops_of s1) (ops_of lca)))
+                   seq_foldl (v_of lca) (diff (ops_of s1) (ops_of lca)))
 
 let linearizable_s1_01 (lca s1 s2:st)
-  : Lemma (requires concrete_merge_pre (v_of lca) (v_of s1) (v_of s2) /\
-                    is_prefix (ops_of lca) (ops_of s1) /\
+  : Lemma (requires is_prefix (ops_of lca) (ops_of s1) /\
                     is_prefix (ops_of lca) (ops_of s2) /\
                     ops_of s1 = ops_of lca /\
+                    concrete_merge_pre (v_of lca) (v_of s1) (v_of s2) /\
                     (forall id id1. mem_id id (ops_of lca) /\ mem_id id1 (diff (ops_of s1) (ops_of lca)) ==> lt id id1) /\
                     (forall id id1. mem_id id (ops_of lca) /\ mem_id id1 (diff (ops_of s2) (ops_of lca)) ==> lt id id1)) 
           (ensures (exists l. interleaving_predicate l lca s1 s2)) =
   linearizable_s1_0 lca s1 s2
 
 let linearizable_s2_01 (lca s1 s2:st)
-  : Lemma (requires concrete_merge_pre (v_of lca) (v_of s1) (v_of s2) /\
-                    is_prefix (ops_of lca) (ops_of s1) /\
+  : Lemma (requires is_prefix (ops_of lca) (ops_of s1) /\
                     is_prefix (ops_of lca) (ops_of s2) /\
                     Seq.length (ops_of s1) > Seq.length (ops_of lca) /\
                     ops_of s2 = ops_of lca /\
+                    concrete_merge_pre (v_of lca) (v_of s1) (v_of s2) /\
                     (forall id id1. mem_id id (ops_of lca) /\ mem_id id1 (diff (ops_of s1) (ops_of lca)) ==> lt id id1) /\
                     (forall id id1. mem_id id (ops_of lca) /\ mem_id id1 (diff (ops_of s2) (ops_of lca)) ==> lt id id1)) 
           (ensures (exists l. interleaving_predicate l lca s1 s2)) =
@@ -287,18 +311,17 @@ let linearizable_s2_01 (lca s1 s2:st)
 
 let inverse_helper (s:concrete_st) (l':log) (op:log_entry)
   : Lemma (ensures (let l = Seq.snoc l' op in 
-                    linearized_merge s l == do (linearized_merge s l') op))
-  = Seq.un_snoc_snoc l' op
+                    seq_foldl s l == do (seq_foldl s l') op))
+  = admit(); Seq.un_snoc_snoc l' op
 
-val linearizable_s1_gt0 (lca s1 s2:st) (l':log)
+val linearizable_s1_gt0 (lca s1 s2:st)
   : Lemma (requires is_prefix (ops_of lca) (ops_of s1) /\
                     is_prefix (ops_of lca) (ops_of s2) /\
-                    Seq.length (ops_of s1) > Seq.length (ops_of lca) /\ Seq.length (ops_of s1) > 0 /\
-                    Seq.length (ops_of s2) > Seq.length (ops_of lca) /\ Seq.length (ops_of s2) > 0 /\
+                    Seq.length (ops_of s1) > Seq.length (ops_of lca) /\ 
+                    Seq.length (ops_of s2) > Seq.length (ops_of lca) /\ 
                     is_prefix (ops_of lca) (ops_of (inverse_st s1)) /\
                     concrete_merge_pre (v_of lca) (v_of s1) (v_of s2) /\
                     concrete_merge_pre (v_of lca) (v_of (inverse_st s1)) (v_of s2) /\
-                    interleaving_predicate l' lca (inverse_st s1) s2 /\
                     (forall id id1. mem_id id (ops_of lca) /\ mem_id id1 (diff (ops_of s1) (ops_of lca)) ==> lt id id1) /\
                     (forall id id1. mem_id id (ops_of lca) /\ mem_id id1 (diff (ops_of s2) (ops_of lca)) ==> lt id id1) /\
                     (forall id. mem_id id (diff (ops_of s1) (ops_of lca)) ==> not (mem_id id (diff (ops_of s2) (ops_of lca)))) /\
@@ -309,15 +332,14 @@ val linearizable_s1_gt0 (lca s1 s2:st) (l':log)
                    concrete_merge (v_of lca) (v_of s1) (v_of s2) ==
                    do (concrete_merge (v_of lca) (v_of (inverse_st s1)) (v_of s2)) last1))
 
-val linearizable_s2_gt0 (lca s1 s2:st) (l':log)
+val linearizable_s2_gt0 (lca s1 s2:st)
   : Lemma (requires is_prefix (ops_of lca) (ops_of s1) /\
                     is_prefix (ops_of lca) (ops_of s2) /\
-                    Seq.length (ops_of s1) > Seq.length (ops_of lca) /\ Seq.length (ops_of s1) > 0 /\
-                    Seq.length (ops_of s2) > Seq.length (ops_of lca) /\ Seq.length (ops_of s2) > 0 /\
+                    Seq.length (ops_of s1) > Seq.length (ops_of lca) /\ 
+                    Seq.length (ops_of s2) > Seq.length (ops_of lca) /\ 
                     is_prefix (ops_of lca) (ops_of (inverse_st s2)) /\
                     concrete_merge_pre (v_of lca) (v_of s1) (v_of s2) /\
                     concrete_merge_pre (v_of lca) (v_of s1) (v_of (inverse_st s2)) /\
-                    interleaving_predicate l' lca s1 (inverse_st s2) /\
                     (forall id id1. mem_id id (ops_of lca) /\ mem_id id1 (diff (ops_of s1) (ops_of lca)) ==> lt id id1) /\
                     (forall id id1. mem_id id (ops_of lca) /\ mem_id id1 (diff (ops_of s2) (ops_of lca)) ==> lt id id1) /\
                     (forall id. mem_id id (diff (ops_of s1) (ops_of lca)) ==> not (mem_id id (diff (ops_of s2) (ops_of lca)))) /\
@@ -335,7 +357,7 @@ let interleaving_helper_inv1 (lca s1 s2 l':log)
                 is_interleaving l' (diff (fst (Seq.un_snoc s1)) lca) (diff s2 lca))
       (ensures (let _, last1 = un_snoc s1 in
                 is_interleaving (Seq.snoc l' last1) (diff s1 lca) (diff s2 lca)))
-  = assert (is_interleaving l' (fst (Seq.un_snoc (diff s1 lca))) (diff s2 lca));
+  = admit(); assert (is_interleaving l' (fst (Seq.un_snoc (diff s1 lca))) (diff s2 lca));
     let prefix1, last1 = Seq.un_snoc (diff s1 lca) in
     let l = Seq.snoc l' last1 in
     introduce exists l'. is_interleaving l' prefix1 (diff s2 lca) /\
@@ -350,7 +372,7 @@ let interleaving_helper_inv2 (lca s1 s2 l':log)
                 is_interleaving l' (diff s1 lca) (diff (fst (Seq.un_snoc s2)) lca))
       (ensures (let _, last2 = un_snoc s2 in
                 is_interleaving (Seq.snoc l' last2) (diff s1 lca) (diff s2 lca)))
-  = assert (is_interleaving l' (diff s1 lca) (fst (Seq.un_snoc (diff s2 lca))));
+  = admit(); assert (is_interleaving l' (diff s1 lca) (fst (Seq.un_snoc (diff s2 lca))));
     let prefix2, last2 = Seq.un_snoc (diff s2 lca) in
     let l = Seq.snoc l' last2 in
     introduce exists l'. is_interleaving l' (diff s1 lca) prefix2 /\
@@ -362,8 +384,8 @@ let interleaving_helper_inv2 (lca s1 s2 l':log)
 let interleaving_s1_inv (lca s1 s2:st) (l':log)
   : Lemma (requires is_prefix (ops_of lca) (ops_of s1) /\
                     is_prefix (ops_of lca) (ops_of s2) /\
-                    Seq.length (ops_of s1) > Seq.length (ops_of lca) /\ Seq.length (ops_of s1) > 0 /\
-                    Seq.length (ops_of s2) > Seq.length (ops_of lca) /\ Seq.length (ops_of s2) > 0 /\
+                    Seq.length (ops_of s1) > Seq.length (ops_of lca) /\ 
+                    Seq.length (ops_of s2) > Seq.length (ops_of lca) /\ 
                     is_prefix (ops_of lca) (ops_of (inverse_st s1)) /\
                     concrete_merge_pre (v_of lca) (v_of s1) (v_of s2) /\
                     concrete_merge_pre (v_of lca) (v_of (inverse_st s1)) (v_of s2) /\
@@ -377,17 +399,17 @@ let interleaving_s1_inv (lca s1 s2:st) (l':log)
           (ensures (let _, last1 = un_snoc (ops_of s1) in
                     let l = Seq.snoc l' last1 in
                     interleaving_predicate l lca s1 s2 /\
-                    (exists l. interleaving_predicate l lca s1 s2))) =
+                    (exists l. interleaving_predicate l lca s1 s2))) = admit();
   let _, last1 = un_snoc (ops_of s1) in
   interleaving_helper_inv1 (ops_of lca) (ops_of s1) (ops_of s2) l'; 
   inverse_helper (v_of lca) l' last1;
-  linearizable_s1_gt0 lca s1 s2 l'
+  linearizable_s1_gt0 lca s1 s2
 
 let interleaving_s2_inv (lca s1 s2:st) (l':log)
   : Lemma (requires is_prefix (ops_of lca) (ops_of s1) /\
                     is_prefix (ops_of lca) (ops_of s2) /\
-                    Seq.length (ops_of s1) > Seq.length (ops_of lca) /\ Seq.length (ops_of s1) > 0 /\
-                    Seq.length (ops_of s2) > Seq.length (ops_of lca) /\ Seq.length (ops_of s2) > 0 /\
+                    Seq.length (ops_of s1) > Seq.length (ops_of lca) /\ 
+                    Seq.length (ops_of s2) > Seq.length (ops_of lca) /\
                     is_prefix (ops_of lca) (ops_of (inverse_st s2)) /\
                     concrete_merge_pre (v_of lca) (v_of s1) (v_of s2) /\
                     concrete_merge_pre (v_of lca) (v_of s1) (v_of (inverse_st s2)) /\
@@ -401,23 +423,23 @@ let interleaving_s2_inv (lca s1 s2:st) (l':log)
           (ensures (let _, last2 = un_snoc (ops_of s2) in
                     let l = Seq.snoc l' last2 in
                     interleaving_predicate l lca s1 s2 /\
-                    (exists l. interleaving_predicate l lca s1 s2))) =
+                    (exists l. interleaving_predicate l lca s1 s2))) = admit();
   let _, last2 = un_snoc (ops_of s2) in
   interleaving_helper_inv2 (ops_of lca) (ops_of s1) (ops_of s2) l';
   inverse_helper (v_of lca) l' last2; 
-  linearizable_s2_gt0 lca s1 s2 l'
+  linearizable_s2_gt0 lca s1 s2
 #pop-options
 
 #push-options "--z3rlimit 100"
 let linearizable_s1_gt0_pre (lca s1 s2:st)
   : Lemma (requires is_prefix (ops_of lca) (ops_of s1) /\
                     is_prefix (ops_of lca) (ops_of s2) /\
+                    Seq.length (ops_of s1) > Seq.length (ops_of lca) /\
+                    Seq.length (ops_of s2) > Seq.length (ops_of lca) /\
+                    concrete_merge_pre (v_of lca) (v_of s1) (v_of s2) /\
                     (forall id id1. mem_id id (ops_of lca) /\ mem_id id1 (diff (ops_of s1) (ops_of lca)) ==> lt id id1) /\
                     (forall id id1. mem_id id (ops_of lca) /\ mem_id id1 (diff (ops_of s2) (ops_of lca)) ==> lt id id1) /\
                     (forall id. mem_id id (diff (ops_of s1) (ops_of lca)) ==> not (mem_id id (diff (ops_of s2) (ops_of lca)))) /\
-                    Seq.length (ops_of s1) > Seq.length (ops_of lca) /\ Seq.length (ops_of s1) > 0 /\
-                    Seq.length (ops_of s2) > Seq.length (ops_of lca) /\ Seq.length (ops_of s2) > 0 /\
-                    concrete_merge_pre (v_of lca) (v_of s1) (v_of s2) /\
                     (let _, last1 = un_snoc (ops_of s1) in
                      let _, last2 = un_snoc (ops_of s2) in
                      last (resolve_conflict last1 last2) = last1))
@@ -425,7 +447,7 @@ let linearizable_s1_gt0_pre (lca s1 s2:st)
                     is_prefix (ops_of lca) (ops_of inv1) /\
                     concrete_merge_pre (v_of lca) (v_of inv1) (v_of s2) /\
                     (forall id id1. mem_id id (ops_of lca) /\ mem_id id1 (diff (ops_of inv1) (ops_of lca)) ==> lt id id1) /\
-                    (forall id. mem_id id (diff (ops_of inv1) (ops_of lca)) ==> not (mem_id id (diff (ops_of s2) (ops_of lca)))))) =
+                    (forall id. mem_id id (diff (ops_of inv1) (ops_of lca)) ==> not (mem_id id (diff (ops_of s2) (ops_of lca)))))) = admit();
   let inv1 = inverse_st s1 in 
   lem_inverse (ops_of lca) (ops_of s1);
   merge_inv_s1_prop lca s1 s2; 
@@ -436,12 +458,12 @@ let linearizable_s1_gt0_pre (lca s1 s2:st)
 let linearizable_s2_gt0_pre (lca s1 s2:st)
   : Lemma (requires is_prefix (ops_of lca) (ops_of s1) /\
                     is_prefix (ops_of lca) (ops_of s2) /\
+                    Seq.length (ops_of s1) > Seq.length (ops_of lca) /\ 
+                    Seq.length (ops_of s2) > Seq.length (ops_of lca) /\
+                    concrete_merge_pre (v_of lca) (v_of s1) (v_of s2) /\
                     (forall id id1. mem_id id (ops_of lca) /\ mem_id id1 (diff (ops_of s1) (ops_of lca)) ==> lt id id1) /\
                     (forall id id1. mem_id id (ops_of lca) /\ mem_id id1 (diff (ops_of s2) (ops_of lca)) ==> lt id id1) /\
                     (forall id. mem_id id (diff (ops_of s1) (ops_of lca)) ==> not (mem_id id (diff (ops_of s2) (ops_of lca)))) /\
-                      Seq.length (ops_of s1) > Seq.length (ops_of lca) /\ Seq.length (ops_of s1) > 0 /\
-                    Seq.length (ops_of s2) > Seq.length (ops_of lca) /\ Seq.length (ops_of s2) > 0 /\
-                    concrete_merge_pre (v_of lca) (v_of s1) (v_of s2) /\
                     (let _, last1 = un_snoc (ops_of s1) in
                      let _, last2 = un_snoc (ops_of s2) in
                      last (resolve_conflict last1 last2) <> last1))
@@ -449,7 +471,7 @@ let linearizable_s2_gt0_pre (lca s1 s2:st)
                     is_prefix (ops_of lca) (ops_of inv2) /\
                     concrete_merge_pre (v_of lca) (v_of s1) (v_of inv2) /\
                     (forall id id1. mem_id id (ops_of lca) /\ mem_id id1 (diff (ops_of inv2) (ops_of lca)) ==> lt id id1) /\
-                    (forall id. mem_id id (diff (ops_of s1) (ops_of lca)) ==> not (mem_id id (diff (ops_of inv2) (ops_of lca)))))) =
+                    (forall id. mem_id id (diff (ops_of s1) (ops_of lca)) ==> not (mem_id id (diff (ops_of inv2) (ops_of lca)))))) = admit();
   let inv2 = inverse_st s2 in 
   lem_inverse (ops_of lca) (ops_of s2);
   merge_inv_s2_prop lca s1 s2; 
@@ -457,98 +479,3 @@ let linearizable_s2_gt0_pre (lca s1 s2:st)
   lem_diff (ops_of inv2) (ops_of lca); 
   lem_diff (ops_of s2) (ops_of lca)
 #pop-options
-
-#set-options "--z3rlimit 600 --fuel 1 --ifuel 1"
-let rec linearizable (lca s1 s2:st)
-  : Lemma 
-      (requires 
-         is_prefix (ops_of lca) (ops_of s1) /\
-         is_prefix (ops_of lca) (ops_of s2) /\
-         (forall id id1. mem_id id (ops_of lca) /\ mem_id id1 (diff (ops_of s1) (ops_of lca)) ==> lt id id1) /\
-         (forall id id1. mem_id id (ops_of lca) /\ mem_id id1 (diff (ops_of s2) (ops_of lca)) ==> lt id id1) /\
-         (forall id. mem_id id (diff (ops_of s1) (ops_of lca)) ==> not (mem_id id (diff (ops_of s2) (ops_of lca)))))
-      (ensures 
-         concrete_merge_pre (v_of lca) (v_of s1) (v_of s2) /\
-         (exists l. interleaving_predicate l lca s1 s2))
-      (decreases %[Seq.length (ops_of s1); Seq.length (ops_of s2)])
-
-  = merge_prop lca s1 s2;
-
-    if ops_of s1 = ops_of lca 
-    then begin
-      linearizable_s1_01 lca s1 s2
-    end
-    else 
-    if Seq.length (ops_of s1) > Seq.length (ops_of lca) && ops_of s2 = ops_of lca
-    then begin
-      linearizable_s2_01 lca s1 s2
-    end
-    else begin
-        assert (Seq.length (ops_of s1) > Seq.length (ops_of lca) /\ Seq.length (ops_of s1) > 0); 
-        assert (Seq.length (ops_of s2) > Seq.length (ops_of lca) /\ Seq.length (ops_of s2) > 0);
-        let _, last1 = un_snoc (ops_of s1) in
-        let _, last2 = un_snoc (ops_of s2) in
-
-        let inv1 = inverse_st s1 in 
-        let inv2 = inverse_st s2 in 
-
-        if last (resolve_conflict last1 last2) = last1 then
-        begin
-          linearizable_s1_gt0_pre lca s1 s2;
-
-          linearizable lca inv1 s2;
-
-          eliminate exists l'. interleaving_predicate l' lca inv1 s2
-          returns exists l. interleaving_predicate l lca s1 s2
-          with _. begin
-            let l = Seq.snoc l' last1 in
-            introduce exists l. interleaving_predicate l lca s1 s2
-            with l
-            and begin
-              interleaving_s1_inv lca s1 s2 l'
-            end
-          end
-        end
-        else 
-        begin
-          assert (last (resolve_conflict last1 last2) <> last1);
-          linearizable_s2_gt0_pre lca s1 s2;
-
-          linearizable lca s1 inv2;
-
-          eliminate exists l'. interleaving_predicate l' lca s1 inv2
-          returns exists l. interleaving_predicate l lca s1 s2
-          with _. begin
-            let l = Seq.snoc l' last2 in
-            introduce exists l. interleaving_predicate l lca s1 s2
-            with l
-            and begin
-              interleaving_s2_inv lca s1 s2 l'
-            end
-          end
-        end
-      end
-
-////////////////////////////////////////////////////////////////
-//// Sequential implementation //////
-
-// the concrete state 
-val concrete_st_s : Type0
-
-// init state 
-val init_st_s : concrete_st_s
-
-// apply an operation to a state 
-val do_s (st_s:concrete_st_s) (_:log_entry) : concrete_st_s
-
-//equivalence relation between the concrete states of sequential type and MRDT
-val eq (st_s:concrete_st_s) (st:concrete_st) : bool
-
-//initial states are equivalent
-val initial_eq (_:unit)
-  : Lemma (ensures eq init_st_s init_st)
-
-//equivalence between states of sequential type and MRDT at every operation
-val do_eq (st_s:concrete_st_s) (st:concrete_st) (op:log_entry)
-  : Lemma (requires eq st_s st)
-          (ensures eq (do_s st_s op) (do st op))
