Increment-only_counter/App.fst
@@ -1,7 +1,9 @@
-module Ictr_inv_b1_b2
+module App
 
 open FStar.Seq
 open FStar.Ghost
+
+#set-options "--query_stats"
 
 // the concrete state type
 // e.g. for the increment only counter (icounter), concrete_st = nat
@@ -17,9 +19,36 @@ type op_t = unit
 // apply an operation to a state
 let do (s:concrete_st) (_:log_entry) : concrete_st = s + 1
 
+////////////////////////////////////////////////////////////////
+//// Sequential implementation //////
+
+// the concrete state 
+type concrete_st_s = nat
+
+// init state 
+let init_st_s = 0
+
+// apply an operation to a state 
+let do_s (s:concrete_st_s) (_:log_entry) : concrete_st_s = s + 1
+
+//equivalence relation between the concrete states of sequential type and MRDT
+let eq (st_s:concrete_st_s) (st:concrete_st) = st_s = st
+
+//initial states are equivalent
+let initial_eq _
+  : Lemma (ensures eq init_st_s init_st) = ()
+
+//equivalence between states of sequential type and MRDT at every operation
+let do_eq (st_s:concrete_st_s) (st:concrete_st) (op:log_entry)
+  : Lemma (requires eq st_s st)
+          (ensures eq (do_s st_s op) (do st op)) 
+  = ()
+
+////////////////////////////////////////////////////////////////
+
 let rec lem_foldl (s:concrete_st) (l:log)
-  : Lemma (ensures ((seq_foldl do s l) = s + length l) /\
-                   (length l > 0 ==> (seq_foldl do s l = seq_foldl do s (fst (un_snoc l)) + 1)))
+  : Lemma (ensures (seq_foldl s l = s + length l) /\
+                   (length l > 0 ==> (seq_foldl s l = seq_foldl s (fst (un_snoc l)) + 1)))
           (decreases length l)
   = match length l with
     |0 -> ()
@@ -71,7 +100,7 @@ let linearizable_s1_0 (lca s1 s2:st)
                 is_prefix (ops_of lca) (ops_of s2) /\
                 ops_of s1 = ops_of lca)
       (ensures concrete_merge (v_of lca) (v_of s1) (v_of s2) == 
-               seq_foldl do (v_of lca) (diff (ops_of s2) (ops_of lca))) =
+               seq_foldl (v_of lca) (diff (ops_of s2) (ops_of lca))) =
   lem_foldl (v_of lca) (diff (ops_of s2) (ops_of lca));
   lem_foldl init_st (ops_of s2);
   lem_foldl init_st (ops_of lca)
@@ -83,60 +112,56 @@ let linearizable_s2_0 (lca s1 s2:st)
                 is_prefix (ops_of lca) (ops_of s2) /\
                 ops_of s2 = ops_of lca)
       (ensures concrete_merge (v_of lca) (v_of s1) (v_of s2) == 
-               seq_foldl do (v_of lca) (diff (ops_of s1) (ops_of lca))) =
+               seq_foldl (v_of lca) (diff (ops_of s1) (ops_of lca))) =
   lem_foldl (v_of lca) (diff (ops_of s1) (ops_of lca));
   lem_foldl init_st (ops_of s1);
   lem_foldl init_st (ops_of lca)
 
-#push-options "--z3rlimit 500"
-let linearizable_s1_gt0 (lca s1 s2:st) (l':log)
+let lem_add (lca s1 s2:nat)
+  : Lemma (ensures s1 - 1 + s2 - lca + 1 = s1 + s2 - lca /\
+                   s1 + (s2 - 1) - lca + 1 = s1 + s2 - lca)
+  = ()
+  
+#push-options "--z3rlimit 100"
+let linearizable_s1_gt0 (lca s1 s2:st)
   : Lemma 
       (requires is_prefix (ops_of lca) (ops_of s1) /\
                 is_prefix (ops_of lca) (ops_of s2) /\
                 Seq.length (ops_of s1) > Seq.length (ops_of lca) /\
                 is_prefix (ops_of lca) (ops_of (inverse_st s1)) /\
                 concrete_merge_pre (v_of lca) (v_of s1) (v_of s2) /\
-                concrete_merge_pre (v_of lca) (v_of (inverse_st s1)) (v_of s2) /\
-                interleaving_predicate l' lca (inverse_st s1) s2)
+                concrete_merge_pre (v_of lca) (v_of (inverse_st s1)) (v_of s2))
       (ensures concrete_merge (v_of lca) (v_of s1) (v_of s2) ==
                do (concrete_merge (v_of lca) (v_of (inverse_st s1)) (v_of s2)) (Seq.last (ops_of s1))) =
-  ()
+  let p1, last1 = un_snoc (ops_of s1) in
+  inverse_helper init_st p1 last1;
+  assert (v_of (inverse_st s1) + v_of s2 - v_of lca =
+          v_of s1 - 1 + v_of s2 - v_of lca);
+  lem_add (v_of lca) (v_of s1) (v_of s2);
+  assert (v_of s1 - 1 + v_of s2 - v_of lca + 1 =
+          v_of s1 + v_of s2 - v_of lca);
+  assert (concrete_merge (v_of lca) (v_of (inverse_st s1)) (v_of s2) + 1 =
+          concrete_merge (v_of lca) (v_of s1) (v_of s2));
+  lem_foldl (v_of lca) (diff (ops_of s1) (ops_of lca))
 
-let linearizable_s2_gt0 (lca s1 s2:st) (l':log)
+let linearizable_s2_gt0 (lca s1 s2:st)
   : Lemma 
       (requires is_prefix (ops_of lca) (ops_of s1) /\
                 is_prefix (ops_of lca) (ops_of s2) /\
                 Seq.length (ops_of s2) > Seq.length (ops_of lca) /\
                 is_prefix (ops_of lca) (ops_of (inverse_st s2)) /\
                 concrete_merge_pre (v_of lca) (v_of s1) (v_of s2) /\
-                concrete_merge_pre (v_of lca) (v_of s1) (v_of (inverse_st s2)) /\
-                interleaving_predicate l' lca s1 (inverse_st s2))
+                concrete_merge_pre (v_of lca) (v_of s1) (v_of (inverse_st s2)))
       (ensures concrete_merge (v_of lca) (v_of s1) (v_of s2) ==
                do (concrete_merge (v_of lca) (v_of s1) (v_of (inverse_st s2))) (Seq.last (ops_of s2))) =
-  ()
+  let p2, last2 = un_snoc (ops_of s2) in
+  inverse_helper init_st p2 last2;
+  assert (v_of s1 + v_of (inverse_st s2) - v_of lca =
+          v_of s1 + (v_of s2 - 1) - v_of lca);
+  lem_add (v_of lca) (v_of s1) (v_of s2);
+  assert (v_of s1 + (v_of s2 - 1) - v_of lca + 1 =
+          v_of s1 + v_of s2 - v_of lca);
+  assert (concrete_merge (v_of lca) (v_of s1) (v_of (inverse_st s2)) + 1 =
+          concrete_merge (v_of lca) (v_of s1) (v_of s2));
+  lem_foldl (v_of lca) (diff (ops_of s2) (ops_of lca))
 #pop-options
-
-////////////////////////////////////////////////////////////////
-//// Sequential implementation //////
-
-// the concrete state 
-type concrete_st_s = nat
-
-// init state 
-let init_st_s = 0
-
-// apply an operation to a state 
-let do_s (s:concrete_st_s) (_:log_entry) : concrete_st_s = s + 1
-
-//equivalence relation between the concrete states of sequential type and MRDT
-let eq (st_s:concrete_st_s) (st:concrete_st) = st_s = st
-
-//initial states are equivalent
-let initial_eq _
-  : Lemma (ensures eq init_st_s init_st) = ()
-
-//equivalence between states of sequential type and MRDT at every operation
-let do_eq (st_s:concrete_st_s) (st:concrete_st) (op:log_entry)
-  : Lemma (requires eq st_s st)
-          (ensures eq (do_s st_s op) (do st op)) 
-  = ()
